extracted identifier class

examples/invariants/DY.Example.Invariants.Uniqueness.Init.fst
@@ -4,73 +4,11 @@ open Comparse
 open DY.Core
 module L = DY.Lib
 open DY.Example.Invariants.Uniqueness
+open DY.Example.Invariants.Uniqueness.Identifier
 
 #set-options "--fuel 1 --ifuel 1"
 
-let prop_state_on (#a:Type) (#state_t:Type) {|ps_state : parseable_serializeable bytes state_t|} 
-  (from_state: state_t  -> a) (p: a -> bool ) (state:state_raw) : prop =
-  match parse state_t state with
-  | None -> True
-  | Some state -> p (from_state state)
-
-let prop_on_idn (f: nat -> bool) (state:state_raw) : prop =
-  prop_state_on
-      (fun state -> state.idn)
-      f
-      state
-
-let forall_idns (f: nat -> bool) (sess:session_raw) : prop =
-  forall_rev_list (prop_on_idn f) sess
-  
-
-let idn_does_not_appear_in_session (idn:nat) (sess:session_raw) : prop =
-  forall_idns (fun idn' -> idn <> idn') sess
-
-val max_id_in_session_largest:
-  sess:session_raw ->
-  Lemma 
-  ( let m_idn = find_max_id_in_session sess in
-    forall_idns (fun idn -> m_idn >= idn) sess
-  )
-let rec max_id_in_session_largest sess = 
-  let m_idn = find_max_id_in_session sess in
-  match sess with
-  | Nil -> ()
-  | Snoc rest state ->
-      max_id_in_session_largest rest
-
-
-
-let idn_does_not_appear_in_full_state (idn:nat) (fst:full_state_raw) : prop =
-  forall_sessions fst (fun sid sess -> idn_does_not_appear_in_session idn sess) 
-
-
-val curr_max_id_largest :
-  fst:full_state_raw ->
-  Lemma 
-  ( let c_max = find_curr_max_id fst in
-    forall_sessions fst (fun sid sess -> forall_idns (fun idn -> c_max >= idn) sess)
-  )
-let rec curr_max_id_largest fst =
-  let c_max = find_curr_max_id fst in
-  match fst with
-  | [] -> ()
-  | (_, sess) :: rest ->
-        max_id_in_session_largest sess;
-        curr_max_id_largest rest
-
-val new_idn_does_not_appear_in_full_state: p:principal -> tr:trace ->
-  Lemma
-  (requires has_full_state_for tr p
-  )
-  (ensures (
-    let (n_idn,_) = new_idn p tr in
-    let fst = access_full_state tr p in
-    n_idn `idn_does_not_appear_in_full_state` fst
-  ))
-let new_idn_does_not_appear_in_full_state p tr =
-  let fst = access_full_state tr p in
-  curr_max_id_largest fst
+(*** Showing that the initial step maintains the trace invariant ***)
 
 #push-options "--z3rlimit 20 --z3cliopt 'smt.qi.eager_threshold=20'"
 val init_invariant: tr:trace -> p:principal ->
@@ -82,16 +20,17 @@ val init_invariant: tr:trace -> p:principal ->
       )
     )
 let init_invariant tr p =
-  let (idn, tr_after_new_idn) = new_idn p tr in
-  let new_state = S idn 0 in
+  let (idn1, tr_after_new_idn1) = new_idn1 p tr in
+  let (idn2, tr_after_new_idn2) = new_idn2 p tr in
+  let new_state = S idn1 idn2 0 in
   let new_state_b = serialize p_state new_state in
-  let (new_sess_id, tr_after_new_session) = set_new_session p (serialize p_state new_state) tr_after_new_idn in
+  let (new_sess_id, _) = set_new_session p new_state_b tr_after_new_idn2 in
   
-  serialize_wf_lemma p_state (is_knowable_by (principal_state_label p new_sess_id) tr_after_new_idn) new_state;
+  serialize_wf_lemma p_state (is_knowable_by (principal_state_label p new_sess_id) tr_after_new_idn2) new_state;
 
-  set_new_session_get_session p (serialize p_state new_state) tr_after_new_idn;
+  set_new_session_get_session p new_state_b tr_after_new_idn2;
 
-  match fst (get_full_state p tr_after_new_idn) with
+  match fst (get_full_state p tr_after_new_idn2) with
   | None -> ()
   | Some full_st ->
       full_state_pred_forall_session_intro full_st new_sess_id
@@ -100,17 +39,17 @@ let init_invariant tr p =
            match parse p_state last_i with
            | None -> True
            | Some last_i ->
-               last_i.idn <> idn
+               last_i.idn1 <> idn1 /\ last_i.idn2 <> idn2
         )
-        (fun sid_i sess_i -> 
+        (fun sid_i sess_i ->
            let Snoc init_ last_i = sess_i in
            match parse p_state last_i with
            | None -> ()
            | Some last_i -> 
-               set_new_session_new_sid p new_state_b tr_after_new_idn;
-               full_state_mem_get_session_get_state_forall p tr_after_new_idn;
-               assert(tr = tr_after_new_idn);
-               new_idn_does_not_appear_in_full_state p tr
+               full_state_mem_get_session_get_state_forall p tr_after_new_idn2;
+               assert(tr = tr_after_new_idn2);
+               new_idn_does_not_appear_in_full_state #p_state #has_identifier_p_state_1 p tr;
+               new_idn_does_not_appear_in_full_state #p_state #has_identifier_p_state_2 p tr
         )
 
 
