examples/invariants/DY.Example.Invariants.Uniqueness.fst
@@ -7,12 +7,19 @@ module Lib = DY.Lib
 module List = FStar.List.Tot.Base
 module Trace = DY.Core.Trace.Type
 
+open DY.Example.Invariants.Uniqueness.Identifier
+
 #set-options "--fuel 1 --ifuel 1"
 
 /// Experimenting with the new state invariants for sessions and full states
 
+/// A state type with two identifiers and a counter.
+/// The idea is that the identifiers are
+/// * the same within a session and
+/// * unique across sessions
+/// and the counter increases in a session
 type p_state =
- | S: idn:nat -> ctr: nat -> p_state
+ | S: idn1:nat -> idn2:nat -> ctr: nat -> p_state
 
 %splice [ps_p_state] (gen_parser (`p_state))
 %splice [ps_p_state_is_well_formed] (gen_is_well_formed_lemma (`p_state))
@@ -20,6 +27,8 @@ type p_state =
 instance parseable_serializeable_bytes_p_state: parseable_serializeable bytes p_state
  = mk_parseable_serializeable ps_p_state
 
+/// some pseudo message and event type
+/// (just to test send message and trigger event)
 
 type message =
   | M: alice:principal -> message
@@ -40,60 +49,78 @@ instance parseable_serializeable_bytes_p_event: parseable_serializeable bytes p_
  = mk_parseable_serializeable ps_p_event
 
 
-let rec find_max_id_in_session (sess:session_raw) : nat = 
-    match sess with
-    | Nil -> 0
-    | Snoc rest state -> 
-        match parse p_state state with
-        | None -> find_max_id_in_session rest
-        | Some (S id _) -> max id (find_max_id_in_session rest)
+/// Saying that idn1 and idn2 are supposed to be identifiers of the state
+/// with this we can call [compute_new_id] for both of them to generate a fresh identifier
+/// and we get the corresponding properties (in particular [new_idn_does_not_appear_in_full_state])
+instance has_identifier_p_state_1: has_identifier p_state = {
+  base = parseable_serializeable_bytes_p_state;
+  to_id = fun state -> state.idn1
+}
 
-let rec find_curr_max_id (st:full_state_raw) : nat = 
-    match st with
-    | [] -> 0
-    | (_,sess)::rest -> max (find_max_id_in_session sess) (find_curr_max_id rest)
+instance has_identifier_p_state_2: has_identifier p_state = {
+  base = parseable_serializeable_bytes_p_state;
+  to_id = fun state -> state.idn2
+}
 
-val new_idn: principal -> traceful nat
-let new_idn prin =
-  let* opt_fst = get_full_state prin in
-  match opt_fst with
-  | None -> return (1 <: nat)
-  | Some fst -> return ((find_curr_max_id fst + 1)<:nat)
+val new_idn1: principal -> traceful nat
+let new_idn1 prin = 
+  compute_new_id #p_state #has_identifier_p_state_1 prin
+
+val new_idn2: principal -> traceful nat
+let new_idn2 prin = 
+  compute_new_id #p_state #has_identifier_p_state_2 prin
 
 
+(*** The Protocol ***)
+
+/// a simple initialization step
+/// that just generates two new ids and sets the counter to 0
 val init: principal -> traceful state_id
 let init prin =
-  let* idn = new_idn prin in
-  let new_state = S idn 0 in
+  let* idn1 = new_idn1 prin in
+  let* idn2 = new_idn2 prin in
+  let new_state = S idn1 idn2  0 in
   let* new_sess_id = set_new_session prin (serialize p_state new_state) in
   return new_sess_id
 
+
+/// a protocol step where
+/// * a state is read,
+/// * a message is sent
+/// * a nonce is generated
+/// * a new state is set in the same session with increased counter
+/// * an event is triggered
+/// * some other state is updated
 val next: principal -> state_id -> traceful (option unit)
 let next prin sid =
   let*? curr_state = get_state prin sid in
-  let*? S idn c = return (parse p_state curr_state) in
+  let*? S idn1 idn2 c = return (parse p_state curr_state) in
   send_msg (serialize message (M prin));*
   let* nonce = mk_rand NoUsage public 7 in
-  set_state prin sid (serialize p_state (S idn (c+1)));*
+  set_state prin sid (serialize p_state (S idn1 idn2 (c+1)));*
   let ev = E prin in
   trigger_event prin "P" (serialize p_event ev);*
 
   let other_sid = {the_id = sid.the_id + 1} in
   let*? other_state = get_state prin other_sid in
-  let*? S other_idn other_c = return (parse p_state other_state) in
-  set_state prin other_sid (serialize p_state (S other_idn (other_c+1)));*
+  let*? S other_idn1 other_idn2 other_c = return (parse p_state other_state) in
+  set_state prin other_sid (serialize p_state (S other_idn1 other_idn2 (other_c+1)));*
   return (Some ())
 
+
+(*** Predicates and Invariants ***)
+
+/// using the default crypto invariants
 let p_cinvs = {
  usages = default_crypto_usages;
  preds = default_crypto_predicates default_crypto_usages
 }
 
-noeq type state_predicate_forall_sessions (cinvs:crypto_invariants) = {
-pred: trace -> principal -> state_id -> state_raw -> prop;
-  session_pred: trace -> session_raw -> principal -> state_id -> state_raw -> prop; 
 
-/// the idea for the new full_state_pred:
+/// Introducing a specialized instance of [state_predicate].
+/// The only difference is in the type of [full_state_pred].
+/// 
+/// The idea is:
 /// often the full_state_pred is of the form:
 /// forall_sessions full_st
 /// (fun sid_i sess_i ->
@@ -108,6 +135,13 @@ pred: trace -> principal -> state_id -> state_raw -> prop;
 /// that hides this form.
 /// That is, when writing such a full_state_pred we can already assume
 /// that sid_i <> sid and Snoc? sess_i
+
+noeq type state_predicate_forall_sessions (cinvs:crypto_invariants) = {
+  pred: trace -> principal -> state_id -> state_raw -> prop;
+  session_pred: trace -> session_raw -> principal -> state_id -> state_raw -> prop; 
+  // notice the new type of the full_state_pred:
+  // the full_state_raw argument is replaced by sid_i and sess_i (an element of the full state)
+  // with the respective restrictions from above
   full_state_pred: trace -> sid_i:state_id -> sess_i:session_raw{Snoc? sess_i} -> principal -> sid:state_id{sid_i <> sid} -> state_raw -> prop;
 
   pred_knowable:
@@ -158,30 +192,33 @@ let f #cinvs sp = {
 }
  
 
+(** The state predicates for this Protocol (using the specialized form of full_state_pred) **)
+
 let p_state_pred: state_predicate_forall_sessions p_cinvs = {
     pred = (fun tr p sid cont -> is_knowable_by #p_cinvs (principal_state_label p sid) tr cont)
   ; session_pred = (fun tr sess prin sid cont ->
-     // within a session the idn should stay the same
+     // within a session the idns should stay the same
      // and the counter must increase
      match parse p_state cont with
      | None -> False
-     | Some (S the_idn the_ctr) -> (
+     | Some (S the_idn1 the_idn2 the_ctr) -> (
          match sess with
          | Nil -> True
          | Snoc init last -> (
              match parse p_state last with
              | None -> True
              | Some last -> 
-                   last.idn = the_idn 
+                   last.idn1 = the_idn1
+                 /\ last.idn2 = the_idn2
                  /\ last.ctr < the_ctr
            )
        )
     )
   ; full_state_pred = (fun tr sid_i sess_i p sid cont -> 
-      // across sessions the idn must be different
+      // across sessions the idns must be different
       match parse p_state cont with
         | None -> False
-        | Some (S the_idn _) -> begin
+        | Some (S the_idn1 the_idn2 _) -> begin
         // using the new full_state_pred
         // we can make use of the fact that
         // sess_i is a Snoc 
@@ -189,7 +226,9 @@ let p_state_pred: state_predicate_forall_sessions p_cinvs = {
             let Snoc _ last_i = sess_i in
             match parse p_state last_i with
             | None -> True
-            | Some last_i -> last_i.idn <> the_idn
+            | Some last_i -> 
+                     last_i.idn1 <> the_idn1
+                   /\ last_i.idn2 <> the_idn2
         end
     )
   ; pred_later = (fun t1 t2 p sid cont -> ())
@@ -200,12 +239,12 @@ let p_state_pred: state_predicate_forall_sessions p_cinvs = {
 instance protocol_invariants_p: protocol_invariants = {
   crypto_invs = p_cinvs;
   trace_invs = {
-    state_pred = f p_state_pred;
+    state_pred = f p_state_pred; // translating to the more general state preds
     event_pred = (fun tr p sid ev -> True)
   }
 }
 
-/// since the new full_state_pred is of the special form,
+/// Since the new full_state_pred is of the special form,
 /// we introduce a convenience function to show such a predicate.
 /// This uses the same structure,
 /// which means that the proof does not need to replicate this structure again.
@@ -216,11 +255,15 @@ instance protocol_invariants_p: protocol_invariants = {
 let full_state_pred_forall_session_intro
   (full_st: full_state_raw) 
   (sid: state_id)
+  // the property on an element of the full state
   (p: (sid_i:state_id{sid_i <> sid}) -> (sess_i:session_raw{Snoc? sess_i}) -> prop)
-  (pf: (sid_i:state_id{sid_i <> sid}) -> (sess_i:session_raw{Snoc? sess_i /\ (sid_i, sess_i) `List.mem` full_st})
+  // a proof of the property under our restrictions
+  (pf: (sid_i:state_id{sid_i <> sid}) -> (sess_i:session_raw{Snoc? sess_i /\ (sid_i, sess_i) `List.memP` full_st})
     -> squash (p sid_i sess_i)
   )
-  : squash (forall_sessions full_st
+  :
+  // shows the generalized [full_state_pred]
+  squash (forall_sessions full_st
     (fun sid_i sess_i ->
     if sid_i = sid || Nil? sess_i
       then True 
@@ -232,6 +275,6 @@ let full_state_pred_forall_session_intro
      sid_i <> sid /\ Snoc? sess_i ==> p sid_i sess_i 
   )
   (fun sid_i sess_i ->
-    introduce (sid_i, sess_i) `List.mem` full_st /\ sid_i <> sid /\ Snoc? sess_i ==> p sid_i sess_i 
+    introduce (sid_i, sess_i) `List.memP` full_st /\ sid_i <> sid /\ Snoc? sess_i ==> p sid_i sess_i 
     with _ . pf sid_i sess_i
   )
