examples/invariants/DY.Example.Invariants.Uniqueness.Identifier.fst
@@ -1,0 +1,139 @@
+module DY.Example.Invariants.Uniqueness.Identifier
+
+open Comparse
+open DY.Core
+module L = DY.Lib
+
+#set-options "--fuel 1 --ifuel 1"
+
+(*** A class for identifiers stored in states ***)
+/// all of this is very similar to [compute_new_session_id]
+
+type session_t #state_t = rev_list state_t
+type full_state_t #state_t = list (state_id * session_t #state_t)
+
+// For now, identifiers are nats.
+// The idea is, that we maybe want to use other things as identifiers as well
+// (for example, randomly generated nonces)
+// If we have appropriate functions and properties to define identifiers,
+// we can make the rest more general.
+// (Ideas so far:
+//  * we need a generating function [compute_new]
+//  * the overall property should be [new_idn_does_not_appear_in_full_state]
+//      * what properties of the generating function do we need for that?
+// )
+type identifier = nat
+
+class has_identifier (state_t:Type) = {
+  base: parseable_serializeable bytes state_t;
+  to_id: state_t -> identifier
+}
+
+
+(*** Generating a new Identifier ***)
+
+let rec find_max_id_in_session (#state_t:Type) {|hid: has_identifier state_t |} 
+    (sess:session_raw) : identifier = 
+    match sess with
+    | Nil -> 0
+    | Snoc rest state -> 
+        match parse state_t #hid.base state with
+        | None -> find_max_id_in_session #state_t rest
+        | Some st ->
+        max (to_id st) (find_max_id_in_session #state_t rest)
+
+
+let rec find_max_id_in_full_state (#state_t:Type) {|hid: has_identifier state_t|}  
+  (st:full_state_raw): identifier = 
+    match st with
+    | [] -> 0
+    | (_,sess)::rest -> 
+        max (find_max_id_in_session #state_t sess) (find_max_id_in_full_state #state_t rest)
+
+val compute_new_id: (#state_t:Type) -> {|hid: has_identifier state_t|} -> principal -> traceful identifier
+let compute_new_id #state_t #hid prin =
+  let* opt_fst = get_full_state prin in
+  match opt_fst with
+  | None -> return (1 <: nat)
+  | Some fst -> 
+        return ((find_max_id_in_full_state #state_t fst + 1)<:nat)
+
+(*** Showing that a newly generated identifier is indeed unique ***)
+
+(** Stating Properties **)
+
+let prop_state_on (#a:Type) (#state_t:Type) {|ps_state : parseable_serializeable bytes state_t|} 
+  (from_state: state_t  -> a) (p: a -> bool ) (state:state_raw) : prop =
+  match parse state_t state with
+  | None -> True
+  | Some state -> p (from_state state)
+
+
+let forall_ids  (#state_t:Type) {|hid:has_identifier state_t|}  
+   (sess:(session_raw)) (p: identifier -> bool) : prop =
+  forall_rev_list sess (fun state -> prop_state_on #_ #state_t #hid.base to_id p state )
+
+
+let id_does_not_appear_in_session (#state_t:Type) {|has_identifier state_t|}  
+  (id:identifier) (sess:session_raw)  : prop =
+  forall_ids #state_t sess (fun id' -> id <> id')
+
+
+let forall_sessions_ (#state_t:Type) (fst:full_state_t) (p:state_id -> session_t #state_t ->  prop)  : prop =
+  forall sid sess. (sid, sess) `List.memP` fst ==> p sid sess
+
+
+let idn_does_not_appear_in_full_state (#state_t:Type) {|has_identifier state_t|}  
+  (id:identifier) (fst:full_state_raw) : prop =
+  forall_sessions fst 
+    (fun _ sess -> id `id_does_not_appear_in_session #state_t` sess)
+
+
+(** Proofs **)
+
+val max_id_in_session_largest:
+  (#state_t:Type) -> {| hid: has_identifier state_t|} ->
+  sess:session_raw ->
+  Lemma 
+  ( let m_idn = find_max_id_in_session #_ #hid sess in
+    forall_ids #state_t sess (fun idn -> m_idn >= idn)
+  )
+let rec max_id_in_session_largest #state_t #hid sess = 
+  let m_idn = find_max_id_in_session #state_t sess in
+  match sess with
+  | Nil -> ()
+  | Snoc rest state ->
+      max_id_in_session_largest #state_t #hid rest
+
+
+val curr_max_id_largest :
+(#state_t:Type) -> {|has_identifier state_t|}  ->
+  (to_id: (state_t -> identifier)) ->
+  fst: full_state_raw -> 
+  Lemma 
+  ( let c_max = find_max_id_in_full_state #state_t fst in
+    forall_sessions fst (fun sid sess -> forall_ids #state_t sess  (fun idn -> c_max >= idn))
+  )
+let rec curr_max_id_largest #state_t to_id fst =
+  let c_max = find_max_id_in_full_state #state_t fst in
+  match fst with
+  | [] -> ()
+  | (_, sess) :: rest ->
+        max_id_in_session_largest #state_t sess;
+        curr_max_id_largest to_id rest
+
+/// The Main Property
+val new_idn_does_not_appear_in_full_state:
+(#state_t:Type) -> {|hid:has_identifier state_t|}  ->
+p:principal -> tr:trace ->
+  Lemma
+  (requires has_full_state_for tr p
+  )
+  (ensures (
+    let (n_id,_) = compute_new_id #state_t p tr in
+    let fst = access_full_state tr p in
+    n_id `idn_does_not_appear_in_full_state #state_t` fst
+  ))
+let new_idn_does_not_appear_in_full_state #state_t #hid p tr =
+  let fst = access_full_state tr p in
+  curr_max_id_largest #state_t to_id fst
