examples/invariants/DY.Example.Invariants.Uniqueness.Next.fst
@@ -11,11 +11,29 @@ open DY.Example.Invariants.Uniqueness
 
 #set-options "--fuel 1 --ifuel 1"
 
+(*** Showing that the [next] protocol step maintains the trace invariant ***)
+
+/// The main Lemma,
+/// saying that the full state predicate is maintained,
+/// when we add a new state to a session with the same idns
+///
+/// The proof looks at every other session (with sid_i <> sid) in the current full state.
+/// The last SetState entry for sid_i comes
+/// either
+///   a) after 
+/// or
+///   b) before
+/// the last SetState entry for sid.
+/// We get that the idns in session sid_i are different from the ones in session sid
+/// by looking at the full state pred at the last SetState entry for
+///   a) sid_i
+/// or
+///   b) sid.
 
 #push-options "--fuel 2 --z3rlimit 20 --z3cliopt 'smt.qi.eager_threshold=20'"
 val state_same_idn_full_state_pred:
   tr:trace -> p:principal -> sid:state_id 
-  -> old_cont:state_raw -> new_cont:state_raw
+  -> new_cont:state_raw
   -> Lemma
     (requires (
          trace_invariant tr
@@ -25,24 +43,25 @@ val state_same_idn_full_state_pred:
           /\ Some? (parse p_state new_cont )
           /\ (let Some old_st = parse p_state old_cont in
              let Some new_st = parse p_state new_cont in
-             old_st.idn = new_st.idn
+               old_st.idn1 = new_st.idn1
+             /\ old_st.idn2 = new_st.idn2
             )
          )
     ))
     (ensures
        full_state_pred tr (access_full_state tr p) p sid new_cont
     )
-let state_same_idn_full_state_pred tr p sid old_cont new_cont =
+let state_same_idn_full_state_pred tr p sid new_cont =
   let old_cont = access_state tr p sid in
   let old_entry = (SetState p sid old_cont) in
-  let Some (S the_idn the_ctr) = parse p_state new_cont in
+  let Some (S the_idn1 the_idn2 the_ctr) = parse p_state new_cont in
 
   full_state_pred_forall_session_intro (access_full_state tr p) sid
   (fun sid_i sess_i ->
     let Snoc _ last_i = sess_i in
          match parse p_state last_i with
          | None -> True
-         | Some last_i -> last_i.idn <> the_idn
+         | Some last_i -> last_i.idn1 <> the_idn1 /\ last_i.idn2 <> the_idn2
   )
   (fun sid_i sess_i ->
      let Snoc _ last_i_b = sess_i in
@@ -85,6 +104,8 @@ let state_same_idn_full_state_pred tr p sid old_cont new_cont =
   )
 #pop-options
 
+
+/// Applying the above lemma to show that [next] maintains the trace invariant
 #push-options "--z3rlimit 50 --z3cliopt 'smt.qi.eager_threshold=50'"
 val next_invariant: tr:trace -> p:principal -> sid:state_id ->
   Lemma 
@@ -100,7 +121,7 @@ let next_invariant tr p sid =
   | (Some oldst_b, _) -> (
       match parse p_state oldst_b with
       | None -> ()
-      | Some (S idn c) -> (          
+      | Some (S idn1 idn2 c) -> (          
           let msg = M p in
           let msg_b = serialize message msg in
           let (_, tr_after_msg) = send_msg msg_b tr in
@@ -108,18 +129,16 @@ let next_invariant tr p sid =
 
           let (_, tr_after_rand) = mk_rand NoUsage public 7 tr_after_msg in
 
-          let next_state = S idn (c+1) in
+          let next_state = S idn1 idn2 (c+1) in
           let next_state_b = serialize p_state next_state in
           let (_,tr_after_next_state) = set_state p sid next_state_b tr_after_rand in
-          
 
           serialize_wf_lemma p_state (is_knowable_by (principal_state_label p sid) tr_after_rand) next_state;
 
           get_state_same p sid tr tr_after_msg;
           get_state_same p sid tr_after_msg tr_after_rand;
 
-          state_same_idn_full_state_pred tr_after_rand p sid oldst_b (serialize p_state (S idn (c+1)));
-
+          state_same_idn_full_state_pred tr_after_rand p sid (serialize p_state (S idn1 idn2 (c+1)));
 
           let ev = E p in
           let ev_b = serialize p_event ev in
@@ -128,20 +147,19 @@ let next_invariant tr p sid =
           let other_sid = {the_id = sid.the_id + 1} in
           match get_state p other_sid tr_after_event with
           | (None, _ ) -> ()
-          | (Some ost_b, _) -> begin
-            match parse p_state ost_b with
-            | None -> ()
-            | Some (S other_idn other_c) ->
-               let other_state = S other_idn (other_c + 1) in
-               let other_state_b = serialize p_state other_state in
-               let (_, tr_after_other_session) = set_state p other_sid other_state_b tr_after_event in
-               
-               parse_wf_lemma #bytes p_state #_ (is_knowable_by (principal_state_label p other_sid) tr_after_event) ost_b;
-               serialize_wf_lemma p_state (is_knowable_by (principal_state_label p other_sid) tr_after_event) other_state;
+          | (Some ost_b, _) -> (
+               match parse p_state ost_b with
+               | None -> ()
+               | Some (S other_idn1 other_idn2 other_c) ->
+                   let other_state = S other_idn1 other_idn2 (other_c + 1) in
+                   let other_state_b = serialize p_state other_state in
+                   let (_, tr_after_other_session) = set_state p other_sid other_state_b tr_after_event in
 
-               state_same_idn_full_state_pred tr_after_event p other_sid ost_b other_state_b
-            end
+                   parse_wf_lemma #bytes p_state #_ (is_knowable_by (principal_state_label p other_sid) tr_after_event) ost_b;
+                   serialize_wf_lemma p_state (is_knowable_by (principal_state_label p other_sid) tr_after_event) other_state;
 
-)
+                   state_same_idn_full_state_pred tr_after_event p other_sid other_state_b
+            )
+        )
     )
 #pop-options
